Queries can now return lists of values. Still need to fix up all the examples.

examples/Trivial.v
@@ -15,6 +15,7 @@ Definition MySchema :=
 Definition Person := TupleDef MySchema "Person".
 Definition Dog := TupleDef MySchema "Dog".
 
+
 Definition MySig : ADTSig :=
   ADTsignature {
     "Empty" : unit → rep,
@@ -37,6 +38,15 @@ Definition MyListImpl_abs
            (nr : list Person * list Dog) : Prop :=
   or!"Person" ≃ fst nr /\ or!"Dog" ≃ snd nr.
 
+Definition People := GetRelationKey MySchema "Person".
+Definition Dogs := GetRelationKey MySchema "Dog".
+
+Definition Age := GetAttributeKey People "Age".
+Definition Name := GetAttributeKey People "Name".
+
+Definition Owner := GetAttributeKey Dogs "Owner".
+Definition Breed := GetAttributeKey Dogs "Breed".
+
 Definition My :
   Sharpened MySpec.
 Proof.
@@ -44,21 +54,75 @@ Proof.
 
   start honing QueryStructure.
 
-  hone method "YoungOwners'Breeds".
-  rewrite Equivalent_Swap_In.
+  (* Need to fix TypeClass lookup for this to go through. *)
+  (* hone method "YoungOwners'Breeds".
+
+
+  etransitivity.
+  setoid_rewrite refine_For_Equivalent_Trace_Ensembles;
+    [ reflexivity
+    | eapply (Equivalent_Swap_In r_n (GetRelationKey MySchema "Dog")
+                                 (GetRelationKey MySchema "Person")
+                                 (fun (d : Dog) (o : Person) =>
+                                    Where (o!"Age" > n)
+                                          Where (d!"Owner" = o!"Name")
+                                          Return d!"Breed"))].
+  etransitivity.
+  setoid_rewrite refine_For_Equivalent_Trace_Ensembles.
+  reflexivity.
+  eapply Equivalent_Under_In; simpl.
+  intros; generalize (Equivalent_Swap_In_Where r_n {|bindex := "Dog" |}
+          (fun (tup : Person) (tup' : Dog) =>
+             Where (tup!"Owner" = tup!"Name")
+                   Return tup'!"Breed")).
+                      ).
   rewrite refine_Query_For_In_Equivalent;
     [ | apply Equivalent_Swap_In_Where with (qs := _)]; cbv beta.
-  finish honing.
+  finish honing. *)
 
   hone representation using MyListImpl_abs.
   implement_empty_list "Empty" MyListImpl_abs.
 
   hone method "YoungOwners'Breeds".
-  unfold MyListImpl_abs in H; split_and.
-  setoid_rewrite refineEquiv_pick_ex_computes_to_and.
-  simplify with monad laws.
-  simpl.
-  setoid_rewrite Equivalent_UnConstr_In_EnsembleListEquivalence;
+  {
+    unfold MyListImpl_abs in H; split_and.
+    setoid_rewrite refineEquiv_pick_ex_computes_to_and.
+    simplify with monad laws.
+    simpl.
+    etransitivity.
+    { setoid_rewrite refine_For_Equivalent_Trace_Ensembles;
+      [ reflexivity | ].
+      eapply (@Equivalent_UnConstr_In_EnsembleListEquivalence 
+                _ _ _ c _
+                (snd r_n)
+                (fun b : Tuple =>
+                   UnConstrQuery_In c People
+                                    (fun o : Person =>
+                                       Where (o Age > n)
+                                             Where (b Owner = o Name)
+                                             Return (b Breed) ))).
+      eauto.
+    }
+    simpl; etransitivity.
+    { apply refine_bind.
+      eapply refine_For_Equivalent_Trace_Ensembles.
+      eapply (@Equivalent_Join_Lists string unit _ _ c People (snd r_n)
+                                 _ (fun el (o : Person) =>
+         Where (o Age > n)
+               Where (el Owner = o Name)
+               Return (el Breed)) H1).
+      unfold pointwise_relation; intros.
+      higher_order_1_reflexivity.
+    } simpl; etransitivity.
+    { apply refine_bind.
+      eapply refine_For_Equivalent_Trace_Ensembles.
+      eapply Equivalent_List_In_Where with (P_dec := _).
+  simpl; intros.
+  eapply X.
+  setoid_rewrite Equivalent_Join_Lists; [ | eassumption ].
+  simpl in X.
+  eapply X.
+  setoid_rewrite Equivalent_UnConstr_In_EnsembleListEquivalence.
     [ | eassumption ].
   setoid_rewrite Equivalent_List_In_Where with (P_dec := _).
   setoid_rewrite Equivalent_Join_Lists; [ | eassumption ].
