src/QueryStructure/QuerySpecs/EnsembleListEquivalence.v
@@ -1,6 +1,7 @@
 Require Import Ensembles List.
 
 Definition EnsembleListEquivalence {A: Type} (ensemble: A -> Prop) (seq: list A) :=
+  NoDup seq /\
   forall x, Ensembles.In _ ensemble x <-> List.In x seq.
 
 Lemma ensemble_list_equivalence_set_eq_morphism {A : Type} {ens1 ens2 : A -> Prop} :
@@ -14,7 +15,7 @@ Proof.
 Qed.
 
 Lemma EnsembleListEquivalence_lift_property {TItem: Type} {P: TItem -> Prop} :
-  forall (sequence: list TItem) (ensemble: TItem -> Prop), 
+  forall (sequence: list TItem) (ensemble: TItem -> Prop),
     EnsembleListEquivalence ensemble sequence ->
     ((forall item,
         List.In item sequence -> P item) <->
@@ -22,7 +23,7 @@ Lemma EnsembleListEquivalence_lift_property {TItem: Type} {P: TItem -> Prop} :
         Ensembles.In _ ensemble item -> P item)).
 Proof.
   intros * equiv;
-  unfold EnsembleListEquivalence in equiv; 
-  setoid_rewrite equiv; 
+  destruct equiv as [NoDup_l equiv];
+  setoid_rewrite equiv;
   reflexivity.
 Qed.
