src/QueryStructure/QuerySpecs/QueryQSSpecs.v
@@ -2,22 +2,35 @@ Require Import List String Ensembles
         Computation.Core
         ADT.ADTSig ADT.Core
         ADTNotation.StringBound ADTNotation.BuildADT ADTNotation.BuildADTSig
-        QueryStructure.QueryStructureSchema  QueryStructure.QueryStructure.
+        QueryStructure.QueryStructureSchema  QueryStructure.QueryStructure
+        EnsembleListEquivalence.
 
-(* Notations for queries. *)
+(* Notations and definitions for queries.
+   The basic idea is to represent queries as ensembles of
+   returned values paired with a trace of the tuples that produced it.
+   [Query_For] projects out the returned values from a list equivalent to
+   this ensemble. Traces are unique since the tuples are pulled from ensembles,
+   guaranteeing the standard SQL semantics.
 
-Definition Query_In (qs : QueryStructureHint) {A} (R : _)
+   If new query syntax is introduced that violates the uniqueness of traces,
+   things might not behave as expected.
+ *)
+
+Open Scope comp.
+
+Definition Query_In (qs : QueryStructureHint) {ReturnT TraceT} (R : _)
            (bod : @Tuple (schemaHeading
-                           (QSGetNRelSchema qsSchemaHint' R)) -> Ensemble A)
-           (a : A) :=
-  exists tup, (GetUnConstrRelation (DropQSConstraints qsHint) R) tup /\
-              bod tup a.
-
+                           (QSGetNRelSchema qsSchemaHint' R))
+                  -> Ensemble (ReturnT * TraceT))
+           (el : ReturnT * (Tuple * TraceT)) :=
+  GetUnConstrRelation (DropQSConstraints qsHint) R (fst (snd el))
+  /\ bod (fst (snd el)) (fst el, snd (snd el)).
 
 Notation "( x 'in' R ) bod" :=
   (Query_In _ {| bindex := R%string |} (fun x => bod)) : QuerySpec_scope.
 
-Definition Query_Return {A : Type} (a a' : A) := (a = a').
+(* [Query_Return] terminates the trace with a unit value. *)
+Definition Query_Return {A : Type} (a : A) (el : A * unit) := (fst el = a).
 
 Notation "'Return' t" :=
   (Query_Return t%Tuple) : QuerySpec_scope.
@@ -29,12 +42,13 @@ Definition Query_Where
 Notation "'Where' p bod" :=
   (Query_Where p%Tuple bod) : QuerySpec_scope.
 
-Definition Query_For
-           {A} (bod : Ensemble A) : Comp (list A) :=
-  Pick (fun l : list A => forall a, (List.In a l) <-> In _ bod a).
+Definition Query_For {ReturnT TraceT}
+           (bod : Ensemble (ReturnT * TraceT)) : Comp (list ReturnT) :=
+  {l | exists l', l = map fst l' /\ EnsembleListEquivalence bod l'}.
 
 Notation "'For' bod" := (Query_For bod) : QuerySpec_scope.
 
 (* The spec for a count of the number of tuples in a relation. *)
 Definition Count {A} (rows : Comp (list A)) : Comp nat :=
-  Bind rows (fun l => ret (List.length l)).
+  l <- rows;
+  ret (List.length l).
