src/QueryStructure/SetEqProperties.v
@@ -1,4 +1,4 @@
-Require Import SetEq Setoid AdditionalLemmas List.
+Require Import SetEq Setoid AdditionalLemmas List Sorting.Permutation.
 
 Definition IsSetEqSafe {A B: Type} (proc: list A -> list B) :=
   forall (seq1 seq2: list A),
@@ -100,13 +100,35 @@ Proof.
 Qed.
 
 Require Import EnsembleListEquivalence.
+Hint Resolve Permutation_in.
+
+Lemma NoDup_Permutation {A} :
+  forall (l l' : list A),
+    Permutation l l' -> NoDup l -> NoDup l'.
+Proof.
+  intros; induction H.
+  + econstructor.
+  + inversion H0; subst; econstructor; eauto.
+    unfold not; intros; apply H3; apply Permutation_sym in H;
+    eapply Permutation_in; eauto.
+  + inversion H0; subst; inversion H3; subst; repeat econstructor; eauto.
+    * unfold not; intros; destruct H; eauto.
+      apply H2; econstructor; eauto.
+    * unfold not; intros; apply H2; econstructor 2; eauto.
+  + eauto.
+Qed.
 
 Add Parametric Morphism {A: Type} (ens: A -> Prop) :
   (EnsembleListEquivalence ens)
-    with signature (@SetEq A ==> @iff)
+    with signature (@Permutation A ==> @iff)
       as ensemble_list_equivalence_morphism.
 Proof.
-  firstorder.
+  firstorder; try eauto using NoDup_Permutation.
+  eapply Permutation_in; eauto; eapply H1; eauto.
+  eapply Permutation_sym in H; eapply H1; eapply Permutation_in; eauto.
+  apply Permutation_sym in H; try eauto using NoDup_Permutation.
+  apply Permutation_sym in H; eapply Permutation_in; eauto; eapply H1; eauto.
+  eapply H1; eapply Permutation_in; eauto.
 Qed.
 
 Add Parametric Morphism {A: Type} :
@@ -118,20 +140,6 @@ Proof.
   setoid_rewrite in_flatten_iff;
   firstorder.
 Qed.
-
-(*
-Require Import State.
-
-Add Parametric Morphism (A: Type) :
-  (State_rect (fun _ => list A))
-    with signature (@SetEq A ==> @SetEq A ==> pointwise_relation _ (@SetEq A))
-      as rect_morphism.
-Proof.
-  intros;
-  unfold pointwise_relation, State_rect;
-  intro state; destruct state; trivial.
-Qed.
-*)
 
 Add Parametric Morphism {A: Type} : (@SetUnion A)
     with signature (@SetEq A ==> @SetEq A ==> @SetEq A)
